code/ecdsa/Hacl.Impl.EC.MontgomeryMultiplication.fst
@@ -18,14 +18,448 @@ open Spec.P256
 open Spec.ECDSA.Lemmas
 
 open Hacl.Impl.EC.LowLevel
+open Hacl.Impl.EC.MontgomeryMultiplication.Lemmas
 
 open Lib.Loops
 open Hacl.Spec.P.MontgomeryMultiplication
 open Hacl.Impl.EC.Setup
 
-(* open Hacl.Impl.P256.MontgomeryMultiplication.Exponent *)
-open Hacl.Impl.P256.MontgomeryMultiplication
-(* open Hacl.Impl.P256.MM.Exponent *)
+
+#set-options "--z3rlimit 200 --fuel 0 --ifuel 0"
+
+
+val montgomery_multiplication_round_: #c: curve -> t: widefelem c -> t2: widefelem c -> 
+  Stack unit
+    (requires fun h -> live h t /\ live h t2 /\ wide_as_nat c h t2 = 0)
+    (ensures fun h0 _ h1 -> modifies (loc t2) h0 h1 /\ 
+      wide_as_nat c h1 t2 < getPower2 c * pow2 64 /\
+      wide_as_nat c h1 t2 = getPrime c * (wide_as_nat c h0 t % pow2 64))
+  
+let montgomery_multiplication_round_ #c t t2 =
+  let t1 = mod64 t in 
+  recall_contents (prime_buffer #c) (Lib.Sequence.of_list (prime_list c)); 
+  short_mul_bn (prime_buffer #c) t1 t2
+  
+
+val montgomery_multiplication_round: #c: curve -> t: widefelem c -> round: widefelem c -> 
+  Stack unit 
+  (requires fun h -> live h t /\ live h round /\ wide_as_nat c h t < getPrime c * getPrime c /\
+    eq_or_disjoint t round)
+  (ensures fun h0 _ h1 -> modifies (loc round)  h0 h1 /\
+    wide_as_nat c h1 round = (wide_as_nat c h0 t + getPrime c * (wide_as_nat c h0 t % pow2 64)) / pow2 64)
+
+let montgomery_multiplication_round #c t round =
+  push_frame(); 
+    let len = getCoordinateLenU64 c in  
+    let t2 = create (size 2 *! len) (u64 0) in 
+    montgomery_multiplication_round_ #c t t2;
+    add_long_without_carry t t2 round;
+    shift1 round round; 
+  pop_frame()  
+
+
+
+#push-options "--z3rlimit 400"
+
+val montgomery_multiplication_round_k0_: #c: curve -> k0: uint64 -> t: widefelem c -> 
+  t2: widefelem c -> 
+  Stack unit
+  (requires fun h -> live h t /\ live h t2 /\ wide_as_nat c h t2 = 0)
+  (ensures fun h0 _ h1 -> modifies (loc t2) h0 h1 /\ 
+    wide_as_nat c h1 t2 < getPower2 c * pow2 64 /\
+    wide_as_nat c h1 t2 = getPrime c * (((wide_as_nat c h0 t % pow2 64) * uint_v k0) % pow2 64))
+
+let montgomery_multiplication_round_k0_ #c k0 t t2 = 
+  push_frame();
+    let t1 = mod64 #c t in
+    
+    let y = create (size 1) (u64 0) in 
+    let temp = create (size 1) (u64 0) in 
+    
+    mul_atomic t1 k0 y temp;
+    recall_contents (prime_buffer #c) (Lib.Sequence.of_list (prime_list c)); 
+
+    let h = ST.get() in 
+    let y_ = index y (size 0) in   
+    modulo_addition_lemma (uint_v (Lib.Sequence.index (as_seq h y) 0)) (pow2 64) (uint_v (Lib.Sequence.index (as_seq h temp) 0));
+    short_mul_bn #c (prime_buffer #c) y_ t2;
+  pop_frame()
+
+
+val montgomery_multiplication_round_k0: #c: curve -> t: widefelem c -> 
+  round: widefelem c -> k0: uint64 ->
+  Stack unit 
+  (requires fun h -> 
+    let prime = getPrime c in 
+    live h t /\ live h round  /\ wide_as_nat c h t < prime * prime)
+  (ensures fun h0 _ h1 -> modifies (loc round) h0 h1 /\ 
+    wide_as_nat c h1 round = (wide_as_nat c h0 t + getPrime c * ((uint_v k0 * (wide_as_nat c h0 t % pow2 64)) % pow2 64)) / pow2 64
+  )
+
+let montgomery_multiplication_round_k0 #c t round k0 = 
+  push_frame(); 
+    let open FStar.Tactics in 
+    let open FStar.Tactics.Canon in 
+    
+    let len = getCoordinateLenU64 c in 
+    let t2 = create (size 2 *! len) (u64 0) in 
+
+    let h0 = ST.get() in 
+    montgomery_multiplication_round_k0_ k0 t t2;
+    
+    assert_by_tactic (getPrime c * (((wide_as_nat c h0 t % pow2 64) * uint_v k0) % pow2 64) == 
+      getPrime c * ((uint_v k0 * (wide_as_nat c h0 t % pow2 64)) % pow2 64)) canon;
+    
+    add_long_without_carry #c t t2 t2; 
+    shift1 #c t2 round;
+  pop_frame()
+
+
+val montgomery_multiplication_buffer_by_one_w_ko: #c: curve {(getPrime c + 1) % pow2 64 == 0} 
+  -> a: felem c
+  -> result: felem c -> 
+  Stack unit
+  (requires (fun h -> live h a /\ as_nat c h a < getPrime c /\ live h result)) 
+  (ensures (fun h0 _ h1 -> modifies (loc result) h0 h1 /\ (let prime = getPrime c in 
+    as_nat c h1 result  = (as_nat c h0 a * modp_inv2_prime (getPower2 c) prime) % prime /\
+    as_nat c h1 result = fromDomain_ #c (as_nat c h0 a)))
+  )
+
+let montgomery_multiplication_buffer_by_one_w_ko #c a result = 
+  push_frame();
+  
+  let len = getCoordinateLenU64 c in 
+  let t = create (size 2 *! len) (u64 0) in 
+    let t_low = sub t (size 0) len in 
+    let t_high = sub t len len in 
+
+  let h0 = ST.get() in 
+
+  copy t_low a; 
+
+  let h1 = ST.get() in 
+  
+  let inv h (i: nat { i <= uint_v (getCoordinateLenU64 c)}) = let prime = getPrime c in 
+    live h t /\ wide_as_nat c h t < prime * prime /\ modifies (loc t) h0 h /\
+    wide_as_nat c h t % prime = wide_as_nat c h1 t * modp_inv2 #c (pow2 (i * 64)) % prime in 
+
+  assert(wide_as_nat c h1 t = as_nat c h0 a + as_nat c h0 t_high * getPower2 c);
+  assert(as_nat c h0 t_high = 0);
+
+  lemma_inv1 (wide_as_nat c h1 t) (getPrime c);
+  lemma_mod_inv #c (wide_as_nat c h1 t);
+
+  let h3 = ST.get() in 
+  for 0ul len inv (fun i ->
+    let h0_ = ST.get() in 
+    montgomery_multiplication_round #c t t; 
+    let h1_ = ST.get() in
+
+
+    let a0 = wide_as_nat c h1 t in 
+    let a_i = wide_as_nat c h0_ t in 
+    let a_il = wide_as_nat c h1_ t in 
+    montgomery_multiplication_one_round_proof_border #c (a_i % pow2 64) a_i a_il;
+    lemma_multiplication_by_inverse_w_k0 #c a0 a_i a_il (v i)
+  );
+
+  let h2 = ST.get() in 
+  
+  assume (wide_as_nat c h2 t < 2 * getPrime c);
+
+  reduction_prime_2prime_with_carry t result;
+  pop_frame();
+  
+  lemmaFromDomain #c (as_nat c h0 a)
+
+
+
+val montgomery_multiplication_buffer_by_one_ko: #c: curve  
+  -> a: felem c
+  -> result: felem c -> 
+  Stack unit
+  (requires (fun h -> live h a /\ as_nat c h a < getPrime c /\ live h result)) 
+  (ensures (fun h0 _ h1 -> modifies (loc result) h0 h1 /\ (
+    let prime = getPrime c in 
+    as_nat c h1 result  = (as_nat c h0 a * modp_inv2_prime (getPower2 c) prime) % prime /\
+    as_nat c h1 result = fromDomain_ #c (as_nat c h0 a)))
+  )
+
+let montgomery_multiplication_buffer_by_one_ko #c a result = 
+  push_frame();
+  
+  let len = getCoordinateLenU64 c in 
+  let t = create (size 2 *! len) (u64 0) in 
+    let t_low = sub t (size 0) len in 
+    let t_high = sub t len len in 
+
+    let h0 = ST.get() in 
+  copy t_low a; 
+    let h1 = ST.get() in 
+    let inv h (i: nat { i <= uint_v (getCoordinateLenU64 c)}) = let prime = getPrime c in 
+      live h t /\ wide_as_nat c h t < prime * prime  /\
+      modifies (loc t) h0 h /\ 
+      wide_as_nat c h t % prime = wide_as_nat c h1 t * modp_inv2 #c (pow2 (i * 64)) % prime
+    in 
+
+    assert(wide_as_nat c h1 t = as_nat c h0 a + as_nat c h0 t_high * getPower2 c);
+    assert(as_nat c h0 t_high = 0);
+
+    lemma_inv1 (wide_as_nat c h1 t) (getPrime c);
+    lemma_mod_inv #c (wide_as_nat c h1 t);
+  
+    for 0ul len inv (fun i -> let h0_ = ST.get() in 
+    montgomery_multiplication_round_k0 #c t t (getKo c); 
+      let h1_ = ST.get() in
+    
+      let a0 = wide_as_nat c h1 t in 
+      let a_i = wide_as_nat c h0_ t in 
+      let a_il = wide_as_nat c h1_ t in 
+
+      montgomery_multiplication_one_round_proof_border #c (v (getKo c) * (a_i % pow2 64) % pow2 64) a_i a_il;
+      lemma_multiplication_by_inverse_k0 #c a0 a_i a_il (v i)
+    );
+      let h2 = ST.get() in 
+  
+      assume (wide_as_nat c h2 t < 2 * getPrime c);
+
+  reduction_prime_2prime_with_carry t result;
+  pop_frame();
+  
+    lemmaFromDomain #c (as_nat c h0 a)
+
+
+val montgomery_multiplication_buffer_w_k0: #c: curve {(getPrime c + 1) % pow2 64 == 0}
+  -> a: felem c -> b: felem c -> result: felem c ->  
+  Stack unit
+  (requires (fun h -> live h a /\ as_nat c h a < getPrime c /\ live h b /\ 
+      live h result /\ as_nat c h b < getPrime c)) 
+  (ensures (fun h0 _ h1 -> modifies (loc result) h0 h1 /\ as_nat c h1 result < getPrime c /\ (
+    let prime = getPrime c in 
+    as_nat c h1 result = (as_nat c h0 a * as_nat c h0 b * modp_inv2_prime (pow2 (getPower c)) prime) % prime /\
+    as_nat c h1 result = toDomain_ #c (fromDomain_ #c (as_nat c h0 a) * fromDomain_ #c (as_nat c h0 b) % prime) /\
+    as_nat c h1 result = toDomain_ #c (fromDomain_ #c (as_nat c h0 a) * fromDomain_ #c (as_nat c h0 b))))
+  )
+
+
+let montgomery_multiplication_buffer_w_k0 #c a b result = 
+  push_frame();
+  let len = getCoordinateLenU64 c in 
+  let t = create (size 2 *! len) (u64 0) in 
+    let h0 = ST.get() in
+  mul a b t;  
+    let h1 = ST.get() in 
+  
+    let inv h (i: nat { i <= uint_v (getCoordinateLenU64 c)}) = let prime = getPrime c in 
+      live h t /\ wide_as_nat c h t < prime * prime /\ modifies (loc t) h0 h /\ 
+      wide_as_nat c h t % prime = wide_as_nat c h1 t * modp_inv2 #c (pow2 (i * 64)) % prime in
+
+    lemma_mult_lt_sqr (as_nat c h0 a) (as_nat c h0 b) (getPrime c);
+    lemma_mod_inv #c (wide_as_nat c h1 t);
+
+  for 0ul len inv (fun i -> let h0_ = ST.get() in
+    montgomery_multiplication_round #c t t; 
+      let h1_ = ST.get() in
+      admit();
+      montgomery_multiplication_one_round_proof_w_ko #c (wide_as_nat c h0_ t) (wide_as_nat c h1_ t) (wide_as_nat c h0_ t)
+    );
+    
+    (*lemma_inv2 #c (wide_as_nat c h1 t) (wide_as_nat c h0_ t) (wide_as_nat c h1_ t) (v i)); *)
+
+    let h2 = ST.get() in 
+  
+    assume (wide_as_nat c h2 t < 2 * getPrime c);
+  reduction_prime_2prime_with_carry t result;
+  
+  pop_frame();
+
+    let prime = getPrime c in 
+    let multResult = as_nat c h0 a * as_nat c h0 b * modp_inv2_prime (pow2 (getPower c)) prime % prime in 
+
+    let a_ = as_nat c h0 a in 
+    let b_ = as_nat c h0 b in 
+    let mod = modp_inv2_prime (pow2 (getPower c)) prime in 
+  
+    calc (==)
+    {
+      a_ * b_ * mod % prime;
+      (==) {lemmaFromDomainToDomain #c multResult}
+      toDomain_ #c (fromDomain_ #c multResult);
+      (==) {lemmaFromDomain #c multResult}
+      toDomain_ #c ((a_ * b_ * mod  % prime) * mod % prime);
+      (==) {lemma_mod_mul_distr_l (a_ * b_ * mod) mod prime}
+      toDomain_ #c (a_ * b_ * mod * mod % prime);
+      (==) {
+	let open FStar.Tactics in 
+	let open FStar.Tactics.Canon in 
+	assert_by_tactic (a_ * b_ * mod * mod == (a_ * mod) * (b_ * mod)) canon}
+      toDomain_ #c ((a_ * mod) * (b_ * mod) % prime);
+      (==) {
+	lemma_mod_mul_distr_l (a_ * mod) (b_ *  mod) prime; 
+	lemma_mod_mul_distr_r (a_ * mod % prime) (b_ * mod) prime}
+      
+      toDomain_ #c ((a_ * mod % prime) * (b_ * mod % prime) % prime);
+      (==) {lemmaFromDomain #c a_; lemmaFromDomain #c b_}
+      toDomain_ #c (fromDomain_ #c a_ * fromDomain_ #c b_ % prime);
+
+    };
+
+    inDomain_mod_is_not_mod #c (fromDomain_ #c a_ * fromDomain_ #c b_)
+
+
+
+val montgomery_multiplication_buffer_k0: #c: curve -> a: felem c -> b: felem c 
+  -> result: felem c ->  
+  Stack unit
+  (requires (fun h -> live h a /\ as_nat c h a < getPrime c /\ live h b /\ 
+    live h result /\ as_nat c h b < getPrime c)) 
+  (ensures (fun h0 _ h1 -> modifies (loc result) h0 h1 /\  
+    as_nat c h1 result < getPrime c /\ (
+    let prime = getPrime c in 
+    as_nat c h1 result = (as_nat c h0 a * as_nat c h0 b * modp_inv2_prime (pow2 (getPower c)) (getPrime c)) % prime /\
+    as_nat c h1 result = toDomain_ #c (fromDomain_ #c (as_nat c h0 a) * fromDomain_ #c (as_nat c h0 b) % prime) /\
+    as_nat c h1 result = toDomain_ #c (fromDomain_ #c (as_nat c h0 a) * fromDomain_ #c (as_nat c h0 b))))
+  )
+
+let montgomery_multiplication_buffer_k0 #c a b result = 
+  push_frame();
+  let len = getCoordinateLenU64 c in 
+  let t = create (size 2 *! len) (u64 0) in 
+    let h0 = ST.get() in 
+  mul a b t;  
+    let h1 = ST.get() in 
+    
+    let inv h (i: nat { i <= uint_v (getCoordinateLenU64 c)}) = let prime = getPrime c in 
+      live h t /\ wide_as_nat c h t < prime * prime /\ modifies (loc t) h0 h /\ 
+      wide_as_nat c h t % prime = wide_as_nat c h1 t * modp_inv2 #c (pow2 (i * 64)) % prime in
+
+    lemma_mult_lt_sqr (as_nat c h0 a) (as_nat c h0 b) (getPrime c);
+    lemma_mod_inv #c (wide_as_nat c h1 t);
+
+    assume (inv h1 0);
+  for 0ul len inv (fun i -> let h0_ = ST.get() in
+    montgomery_multiplication_round_k0 #c t t (getKo c); 
+      let h1_ = ST.get() in
+      admit();
+      montgomery_multiplication_one_round_proof_w_ko #c (wide_as_nat c h0_ t) (wide_as_nat c h1_ t) (wide_as_nat c h0_ t)
+      (*lemma_inv2 #c (wide_as_nat c h1 t) (wide_as_nat c h0_ t) (wide_as_nat c h1_ t) (v i) *));
+
+    let h2 = ST.get() in   
+    assume (wide_as_nat c h2 t < 2 * getPrime c);
+  reduction_prime_2prime_with_carry t result;
+  
+  pop_frame();
+
+    let prime = getPrime c in 
+    let multResult = as_nat c h0 a * as_nat c h0 b * modp_inv2_prime (pow2 (getPower c)) prime % prime in 
+
+    let a_ = as_nat c h0 a in 
+    let b_ = as_nat c h0 b in 
+    let mod = modp_inv2_prime (pow2 (getPower c)) prime in 
+
+    admit();
+    calc (==)
+    {
+      a_ * b_ * mod % prime;
+      (==) {lemmaFromDomainToDomain #c multResult}
+      toDomain_ #c (fromDomain_ #c multResult);
+      (==) {lemmaFromDomain #c multResult}
+      toDomain_ #c ((a_ * b_ * mod  % prime) * mod % prime);
+      (==) {lemma_mod_mul_distr_l (a_ * b_ * mod) mod prime}
+      toDomain_ #c (a_ * b_ * mod * mod % prime);
+      (==) {
+	let open FStar.Tactics in 
+	let open FStar.Tactics.Canon in 
+	assert_by_tactic (a_ * b_ * mod * mod == (a_ * mod) * (b_ * mod)) canon}
+      toDomain_ #c ((a_ * mod) * (b_ * mod) % prime);
+      (==) {
+	lemma_mod_mul_distr_l (a_ * mod) (b_ *  mod) prime; 
+	lemma_mod_mul_distr_r (a_ * mod % prime) (b_ * mod) prime}
+      
+      toDomain_ #c ((a_ * mod % prime) * (b_ * mod % prime) % prime);
+      (==) {lemmaFromDomain #c a_; lemmaFromDomain #c b_}
+      toDomain_ #c (fromDomain_ #c a_ * fromDomain_ #c b_ % prime);
+
+    };
+
+    inDomain_mod_is_not_mod #c (fromDomain_ #c a_ * fromDomain_ #c b_)
+
+
+
+val montgomery_square_buffer_w_k0: #c: curve {(getPrime c + 1) % pow2 64 == 0} -> a: felem c
+  -> result: felem c ->  
+  Stack unit
+  (requires (fun h -> live h a /\ as_nat c h a < (getPrime c) /\ live h result)) 
+  (ensures (fun h0 _ h1 -> (let prime = getPrime c in modifies (loc result) h0 h1 /\  
+    as_nat c h1 result < prime /\ 
+    as_nat c h1 result = (as_nat c h0 a * as_nat c h0 a * modp_inv2_prime (getPower c) prime) % prime /\
+    as_nat c h1 result = toDomain_ #c (fromDomain_ #c (as_nat c h0 a) * fromDomain_ #c (as_nat c h0 a) % prime) /\
+    as_nat c h1 result = toDomain_ #c (fromDomain_ #c (as_nat c h0 a) * fromDomain_ #c (as_nat c h0 a)))))
+
+
+let montgomery_square_buffer_w_k0 #c a result = 
+  push_frame();
+    
+  let len = getCoordinateLenU64 c in 
+  let t = create (size 2 *! len) (u64 0) in 
+    let h0 = ST.get() in 
+  square_bn a t;  
+    let h1 = ST.get() in 
+  let inv h (i: nat { i <= uint_v len}) =  let prime = getPrime c in 
+    live h t /\ wide_as_nat c h t < prime * prime  /\
+    modifies (loc t) h0 h /\
+    wide_as_nat c h t % prime = wide_as_nat c h1 t * modp_inv2 #c (pow2 (i * 64)) % prime in 
+
+    assume (wide_as_nat c h1 t < getPrime c * getPrime c);
+    assume (wide_as_nat c h1 t % getPrime c = wide_as_nat c h1 t * modp_inv2 #c (pow2 (0 * 64)) % getPrime c);
+  
+  for 0ul len inv (fun i ->
+      let h0_ = ST.get() in 
+    montgomery_multiplication_round #c t t; 
+      let h1_ = ST.get() in
+
+      let a0 = wide_as_nat c h1 t in 
+      let a_i = wide_as_nat c h0_ t in 
+      let a_il = wide_as_nat c h1_ t in 
+      montgomery_multiplication_one_round_proof_border #c (a_i % pow2 64) a_i a_il;
+      lemma_multiplication_by_inverse_w_k0 #c a0 a_i a_il (v i));
+
+    let h2 = ST.get() in 
+    assume (wide_as_nat c h2 t < 2 * getPrime c);
+  reduction_prime_2prime_with_carry t result; 
+    admit();
+    
+  pop_frame()  
+
+
+
+val montgomery_square_buffer_k0: #c: curve -> a: felem c -> result: felem c ->  
+  Stack unit
+  (requires (fun h -> live h a /\ as_nat c h a < getPrime c /\ live h result)) 
+  (ensures (fun h0 _ h1 -> (modifies (loc result) h0 h1 /\ (let prime = getPrime c in 
+    as_nat c h1 result < prime /\ 
+    as_nat c h1 result = (as_nat c h0 a * as_nat c h0 a * modp_inv2_prime (getPower c) prime) % prime /\
+    as_nat c h1 result = toDomain_ #c (fromDomain_ #c (as_nat c h0 a) * fromDomain_ #c (as_nat c h0 a) % prime) /\
+    as_nat c h1 result = toDomain_ #c (fromDomain_ #c (as_nat c h0 a) * fromDomain_ #c (as_nat c h0 a)))))
+  )
+
+
+let montgomery_square_buffer_k0 #c a result = 
+  push_frame();
+    
+  let len = getCoordinateLenU64 c in 
+  let t = create (size 2 *! len) (u64 0) in 
+    let h0 = ST.get() in 
+  square_bn a t;  
+    let h1 = ST.get() in 
+  let inv h (i: nat { i <= uint_v len}) = True in 
+    for 0ul len inv (fun i -> montgomery_multiplication_round_k0 #c t t (getKo c));
+
+  reduction_prime_2prime_with_carry t result; 
+  admit();
+   
+  pop_frame()  
+
 
 inline_for_extraction
 val supportsReducedMultiplication: #c: curve -> 
@@ -43,26 +477,23 @@ let supportsReducedMultiplication #c =
 let montgomery_multiplication_buffer_by_one #c a result = 
   match supportsReducedMultiplication #c with 
   |true -> 
-   (* assume ((getPrime c + 1) % pow2 64 == 0); *)
     montgomery_multiplication_buffer_by_one_w_ko a result
   |false -> montgomery_multiplication_buffer_by_one_ko a result
 
 
 let montgomery_multiplication_buffer #c a b result = 
-  match c with 
-  |P256 ->
-    assume ((getPrime c + 1) % pow2 64 == 0);
+  match supportsReducedMultiplication #c with 
+  |true -> 
     montgomery_multiplication_buffer_w_k0 a b result
-  |P384 -> montgomery_multiplication_buffer_k0 a b result
+  |false -> montgomery_multiplication_buffer_k0 a b result
 
 
 
 let montgomery_square_buffer #c a result = 
-  match c with 
-  |P256 ->
-     assume ((getPrime c + 1) % pow2 64 == 0);
+  match supportsReducedMultiplication #c with 
+  |true -> 
      montgomery_square_buffer_w_k0 a result
-  |P384 -> montgomery_square_buffer_k0 a result
+  |false -> montgomery_square_buffer_k0 a result
 
 
 
