code/ecdsa/Hacl.Impl.EC.MontgomeryMultiplication.Lemmas.fst
@@ -1,0 +1,223 @@
+module Hacl.Impl.EC.MontgomeryMultiplication.Lemmas
+
+
+open FStar.HyperStack.All
+open FStar.HyperStack
+module ST = FStar.HyperStack.ST
+
+open Hacl.Impl.P256.Math 
+
+open Lib.IntTypes
+open Lib.Buffer
+
+open FStar.Math.Lemmas
+open FStar.Mul
+
+open Hacl.Spec.P256.Definition
+open Hacl.Lemmas.P256
+open Spec.P256
+open Spec.ECDSA.Lemmas
+
+open Hacl.Impl.EC.LowLevel
+
+open Lib.Loops
+open Hacl.Spec.P.MontgomeryMultiplication
+open Hacl.Impl.EC.Setup
+
+
+
+
+
+
+val lemma_add_lt: a : int -> b: int -> q: int -> q1: int -> Lemma
+  (requires (a < q /\ b < q1))
+  (ensures (a + b < q + q1))
+
+let lemma_add_lt a b q q1 = ()
+
+val lemma_one_round_0: a: nat -> b1: nat -> b2: nat -> Lemma 
+  (requires (a <= (b1 + pow2 64 * b2) / pow2 64))
+  (ensures (a <= b1 / pow2 64 + b2))
+
+let lemma_one_round_0 a b1 b2 =
+  lemma_div_plus b1 b2 (pow2 64)
+
+
+
+val montgomery_multiplication_one_round_proof_border: #c: curve ->
+  z: nat {z < pow2 64} -> 
+  t: nat {t < getPrime c * getPrime c} -> 
+  result: nat {result = (t + getPrime c * z) / pow2 64} ->
+  Lemma
+    (result < getPrime c * getPrime c)
+
+
+let montgomery_multiplication_one_round_proof_border #c z t result  = 
+  let prime = getPrime c in 
+  lemma_mult_lt_right prime z (pow2 64)
+
+
+val montgomery_multiplication_one_round_proof_w_ko: 
+  #c: curve {(getPrime c + 1) % pow2 64 == 0} ->
+  t: nat {t < getPrime c * getPrime c} -> 
+  result: nat {result = (t + getPrime c * (t % pow2 64)) / pow2 64} ->
+  co: nat {co % getPrime c == t % getPrime c} -> 
+  Lemma (
+    result % getPrime c == co * modp_inv2 #c (pow2 64) % getPrime c)
+
+
+let montgomery_multiplication_one_round_proof_w_ko #c t result co = 
+  let prime = getPrime c in 
+  mult_one_round #c t co; 
+  mul_lemma_1 (t % pow2 64) (pow2 64) prime; 
+  
+  lemma_mult_lt_sqr prime prime (getPower2 c);
+  lemma_mult_lt_left (pow2 64) prime (getPower2 c);
+  lemma_add_lt (prime * prime) (pow2 64 * prime) (getPower2 c * getPower2 c) (pow2 64 * getPower2 c)
+
+
+val lemma_mod_inv: #c: curve ->  t: int -> Lemma (t % getPrime c = t * modp_inv2 #c (pow2 0) % getPrime c)
+
+let lemma_mod_inv #c t = 
+  let prime = getPrime c in 
+  lemma_pow_mod_n_is_fpow prime 1 (prime - 2);
+  power_one (prime - 2)
+
+
+val lemma_inv1: a: int -> b: int{a < b} -> Lemma (a < b * b)
+
+let lemma_inv1 a b = ()
+
+
+val lemma_modp_as_pow: #c: curve -> a: nat -> Lemma
+    (modp_inv2 #c a == pow (a % getPrime c) (getPrime c - 2) % getPrime c)
+
+let lemma_modp_as_pow #c a = 
+  let prime = getPrime c in 
+  lemma_pow_mod_n_is_fpow prime (a % prime) (prime - 2)
+
+
+val lemma_multiplication_by_inverse_w_k0: #c: curve{(getPrime c + 1) % pow2 64 == 0} 
+  -> a0: nat -> a_i: nat {a_i < getPrime c * getPrime c} 
+  -> a_i1: nat {a_i1 = (a_i + getPrime c * (a_i % pow2 64)) / pow2 64} 
+  -> i: nat {i < uint_v (getCoordinateLenU64 c)} -> 
+  Lemma 
+    (requires (a_i % getPrime c = a0 * modp_inv2 #c (pow2 (i * 64)) % getPrime c))
+    (ensures (a_i1 % getPrime c = a0 * modp_inv2 #c (pow2 ((i + 1) * 64)) % getPrime c))
+
+
+let lemma_multiplication_by_inverse_w_k0 #c a0 a_i a_i1 i = 
+  let prime = getPrime c in 
+
+  let open FStar.Tactics in 
+  let open FStar.Tactics.Canon in 
+ 
+  assert_by_tactic (a0 * (modp_inv2 #c (pow2 (i * 64))) * (modp_inv2 #c (pow2 64)) == a0 * ((modp_inv2 #c (pow2 (i * 64))) * (modp_inv2 #c (pow2 64)))) canon;
+ 
+  montgomery_multiplication_one_round_proof_w_ko #c a_i a_i1 (a0 * modp_inv2 #c (pow2 (i * 64)));
+  lemma_mod_mul_distr_r a0 (modp_inv2 #c (pow2 (i * 64)) * modp_inv2 #c (pow2 64)) prime;
+
+
+  let pow2_64 = pow2 64 in 
+
+  calc(==)
+  {
+    modp_inv2 #c (pow2 (i * 64)) * modp_inv2 #c pow2_64 % prime;
+    (==) {lemma_modp_as_pow #c (pow2 (i * 64)); lemma_modp_as_pow #c pow2_64}
+    (pow (pow2_64 % prime) (prime - 2) % prime) * (pow (pow2 (i * 64) % prime) (prime - 2) % prime) % prime;
+    (==) {power_distributivity (pow2_64) (prime - 2) prime}
+    (pow (pow2_64) (prime - 2) % prime) * (pow (pow2 (i * 64) % prime) (prime - 2) % prime) % prime;
+    (==) {power_distributivity (pow2 (i * 64)) (prime - 2) prime}
+    (pow (pow2_64) (prime - 2) % prime) * (pow (pow2 (i * 64)) (prime - 2) % prime) % prime;
+    (==) {lemma_mod_mul_distr_l (pow (pow2_64) (prime - 2)) (pow (pow2 (i * 64)) (prime - 2) % prime) prime}
+    (pow (pow2_64) (prime - 2)) * (pow (pow2 (i * 64)) (prime - 2) % prime) % prime;
+    (==) {lemma_mod_mul_distr_r (pow (pow2_64) (prime - 2)) (pow (pow2 (i * 64)) (prime - 2)) prime}
+    (pow (pow2_64) (prime - 2)) * (pow (pow2 (i * 64)) (prime - 2)) % prime;
+    (==) {power_distributivity_2 pow2_64 (pow2 (i * 64)) (prime - 2)}
+    (pow (pow2_64 * pow2 (i * 64)) (prime - 2)) % prime;
+    (==) {pow2_plus 64 (i * 64)}
+    (pow (pow2 ((i + 1) * 64)) (prime - 2)) % prime; 
+    (==) {power_distributivity (pow2 ((i + 1) * 64)) (prime - 2) prime}
+    (pow (pow2 ((i + 1) * 64) % prime) (prime - 2)) % prime; 
+    (==) {lemma_modp_as_pow #c (pow2 ((i + 1) * 64))}
+    modp_inv2 #c (pow2 ((i + 1) * 64)); 
+    
+    }
+
+
+val lemma_reduce_mod_ecdsa_prime:
+  #c: curve 
+  -> t: nat 
+  -> k0: nat {k0 = min_one_prime (pow2 64) (- getPrime c)} ->  Lemma (
+    let prime = getPrime c in 
+    (t + prime * (k0 * (t % pow2 64) % pow2 64)) % pow2 64 == 0)
+    
+let lemma_reduce_mod_ecdsa_prime #c t k0 = 
+  let prime = getPrime c in 
+
+  assert_norm(exp #(pow2 64) ((- getPrime P384) % pow2 64) ( pow2 64) == 1);
+  admit()
+
+
+(*
+  let f = prime * (k0 * (t % pow2 64) % pow2 64) in 
+  let t0 = (t + f) % pow2 64 in 
+  lemma_mod_add_distr t f (pow2 64);
+  modulo_addition_lemma t (pow2 64) f;
+  lemma_mod_mul_distr_r k0 t (pow2 64);
+  lemma_mod_mul_distr_r prime (k0 * t) (pow2 64); 
+    assert_by_tactic(prime * (k0 * t) == (prime * k0) * t) canon;
+  lemma_mod_mul_distr_l (prime * k0) t (pow2 64); 
+    assert_norm (exp #(pow2 64) 884452912994769583 (pow2 64  - 1)  = 14758798090332847183);
+  lemma_mod_mul_distr_l (-1) t (pow2 64);
+  lemma_mod_add_distr t (-t) (pow2 64) *)
+
+
+val mult_one_round_ecdsa_prime: 
+  #c: curve 
+  -> t: nat 
+  -> co: nat {t % getPrime c == co % getPrime c} 
+  -> k0: nat {k0 = min_one_prime (pow2 64) (- getPrime c)} -> 
+  Lemma (
+    let prime = getPrime c in 
+    let result = (t + getPrime c * ((k0 * (t % pow2 64)) % pow2 64)) / pow2 64 in 
+    result % prime == (co * modp_inv2_prime (pow2 64) prime) % prime)
+
+
+let mult_one_round_ecdsa_prime #c t co k0 = 
+  let prime = getPrime c in 
+  
+  let t2 = ((k0 * (t % pow2 64)) % pow2 64) * prime in 
+  let t3 = t + t2 in  
+
+  modulo_addition_lemma t prime ((k0 * (t % pow2 64)) % pow2 64); 
+  lemma_div_mod t3 (pow2 64);
+  (*admit();
+  lemma_reduce_mod_ecdsa_prime prime t k0;
+  admit(); *)
+  admit();
+      assert(let rem = t3/ pow2 64 in rem * pow2 64 = t3);
+      assert(exists (k: nat). k * pow2 64 = t3);
+    lemma_division_is_multiplication t3 prime;
+    lemma_multiplication_to_same_number t3 co (modp_inv2_prime (pow2 64) prime) prime
+
+
+val lemma_multiplication_by_inverse_k0: 
+    #c: curve
+  -> a0: nat 
+  -> a_i: nat {a_i < getPrime c * getPrime c} 
+  -> a_i1: nat {a_i1 = (a_i + getPrime c * ((v (getKo c) * (a_i % pow2 64)) % pow2 64)) / pow2 64} 
+  -> i: nat {i < uint_v (getCoordinateLenU64 c)} -> 
+  Lemma 
+    (requires (a_i % getPrime c = a0 * modp_inv2 #c (pow2 (i * 64)) % getPrime c))
+    (ensures (a_i1 % getPrime c = a0 * modp_inv2 #c (pow2 ((i + 1) * 64)) % getPrime c))
+
+
+let lemma_multiplication_by_inverse_k0 #c a0 a_i a_i1 i = 
+  assert(a_i % getPrime c == a0 * modp_inv2 #c (pow2 (i * 64)) % getPrime c);
+  assert(a_i1 =  (a_i + getPrime c * ((v (getKo c) * (a_i % pow2 64)) % pow2 64)) / pow2 64);
+
+  assert(v (getKo c) = min_one_prime (pow2 64) (- getPrime c));
+
+  admit()
+
